finished user integrity proof

InvIfScript.sml
@@ -13,11 +13,13 @@ val _ = new_theory "InvIf";
 
 val CR_exists = prove (``
 ?CR:core_state # mem_view -> resource set.
-!c c' mv mv'. (!r. r IN CR(c,mv) ==> (CV c mv r = CV c' mv' r)) ==>
-	      (CR(c,mv) = CR(c',mv'))
+!c c' mv mv'. ((!r. r IN CR(c,mv) ==> (CV c mv r = CV c' mv' r)) ==>
+	       (CR(c,mv) = CR(c',mv')))
+	   /\ (!r. reg_res r /\ r IN CR(c,mv) ==> ?r'. r = COREG r')
 ``,
   EXISTS_TAC ``\ (c,mv):core_state # mem_view. EMPTY:resource set`` >>
-  RW_TAC std_ss []
+  RW_TAC std_ss [] >>
+  FULL_SIMP_TAC std_ss [pred_setTheory.NOT_IN_EMPTY]
 );  
 
 val CR_spec = new_specification ("CR_spec",
@@ -37,7 +39,17 @@ val CR_oblg = store_thm("CR_oblg", ``
   IMP_RES_TAC CR_spec
 );
 
-val CRex_oblg = store_thm("CR_oblg", ``
+val CR_coreg_oblg = store_thm("CR_coreg_oblg", ``
+!s s' r. reg_res r /\ r IN CR s /\ (s'.cs.coreg = s.cs.coreg) ==> 
+    (Cv s r = Cv s' r) 
+``,
+  REPEAT STRIP_TAC >>
+  FULL_SIMP_TAC std_ss [CR_def] >>
+  IMP_RES_TAC CR_spec >>
+  RW_TAC std_ss [Cv_def, coreIfTheory.CV_def]
+);
+
+val CRex_oblg = store_thm("CRex_oblg", ``
 !s r. r IN CRex s ==> (?pa. (r = MEM pa)) /\ r IN CR s /\ ?m. Mon s r m EX
 ``,
   RW_TAC std_ss [CRex_def] >> (
@@ -72,6 +84,26 @@ val Icoh_CR_po = Define `Icoh_CR_po I =
 
 val Icoh_dCoh_po = Define `Icoh_dCoh_po I = 
 !s. I s ==> dCoh s.ms {pa | MEM pa IN CR s}
+`;
+
+val Icode_CR_po = Define `Icode_CR_po I = 
+!s s'. dCoh s.ms {pa | MEM pa IN CR s} 
+    /\ dCoh s'.ms {pa | MEM pa IN CR s'}
+    /\ iCoh s.ms {pa | MEM pa IN CRex s}
+    /\ iCoh s'.ms {pa | MEM pa IN CRex s'}
+    /\ isafe s {pa | MEM pa IN CRex s}
+    /\ isafe s' {pa | MEM pa IN CRex s'}
+    /\ (!r. r IN CR s ==> (Cv s r = Cv s' r))
+        ==>
+    (I s <=> I s')
+`;
+
+val Icode_iCoh_po = Define `Icode_iCoh_po I = 
+!s. I s ==> iCoh s.ms {pa | MEM pa IN CRex s}
+`;
+
+val Icode_isafe_po = Define `Icode_isafe_po I = 
+!s. I s ==> isafe s {pa | MEM pa IN CRex s}
 `;
 
 val Icm_po = Define `Icm_po I Icm =
@@ -109,31 +141,42 @@ val Ifun_exists = store_thm("Ifun_exists", ``
 );
 
 val Icoh_exists = store_thm("Icoh_exists", ``
-?Icoh. Icoh_CR_po Icoh /\ Icoh_dCoh_po Icoh
+?Icoh. Icoh_CR_po Icoh /\ Icoh_dCoh_po Icoh 
 ``,
   EXISTS_TAC ``\s. dCoh s.ms {pa | MEM pa IN CR s}`` >>
   RW_TAC std_ss [Icoh_dCoh_po, Icoh_CR_po]
 );
 
+val Icode_exists = store_thm("Icoh_exists", ``
+?Icode. Icode_CR_po Icode /\ Icode_iCoh_po Icode /\ Icode_isafe_po Icode
+``,
+  EXISTS_TAC ``\s. iCoh s.ms {pa | MEM pa IN CRex s}
+                /\ isafe s {pa | MEM pa IN CRex s}`` >>
+  RW_TAC std_ss [Icode_CR_po, Icode_iCoh_po, Icode_isafe_po]
+);
+
 val Inv_exists = store_thm("Inv_exists", ``
-?Inv Ifun Icoh Icm.
-    (!s. Inv s <=> Ifun s /\ Icoh s /\ Icm s)
+?Inv Ifun Icoh Icode Icm.
+    (!s. Inv s <=> Ifun s /\ Icoh s /\ Icode s /\ Icm s)
  /\ Ifun_CR_po Ifun /\ Ifun_MD_po Ifun /\ Ifun_Mon_po Ifun
  /\ Icoh_CR_po Icoh /\ Icoh_dCoh_po Icoh
+ /\ Icode_CR_po Icode /\ Icode_iCoh_po Icode /\ Icode_isafe_po Icode
  /\ Icm_po Inv Icm
 ``,
   ASSUME_TAC Ifun_exists >>
   ASSUME_TAC Icoh_exists >>
+  ASSUME_TAC Icode_exists >>
   FULL_SIMP_TAC std_ss [] >>
-  EXISTS_TAC ``\s:hw_state. Ifun s /\ Icoh s`` >>
+  EXISTS_TAC ``\s:hw_state. Ifun s /\ Icoh s /\ Icode s`` >>
   EXISTS_TAC ``Ifun:hw_state -> bool`` >>
   EXISTS_TAC ``Icoh:hw_state -> bool`` >>
+  EXISTS_TAC ``Icode:hw_state -> bool`` >>
   EXISTS_TAC ``\s:hw_state. T`` >>
   RW_TAC std_ss [Icm_po]
 );
 
 val Inv_spec = new_specification ("Inv_spec",
-  ["Inv", "Ifun", "Icoh", "Icm"], Inv_exists);
+  ["Inv", "Ifun", "Icoh", "Icode", "Icm"], Inv_exists);
 
 (* exported theorems *)
 
@@ -188,6 +231,41 @@ val Icoh_dCoh_oblg = store_thm("Icoh_dCoh_oblg", ``
   IMP_RES_TAC Icoh_dCoh_po 
 ); 
 
+val Icode_CR_oblg = store_thm("Icode_CR_oblg", ``
+!s s'. dCoh s.ms {pa | MEM pa IN CR s} 
+    /\ dCoh s'.ms {pa | MEM pa IN CR s'}
+    /\ iCoh s.ms {pa | MEM pa IN CRex s}
+    /\ iCoh s'.ms {pa | MEM pa IN CRex s'}
+    /\ isafe s {pa | MEM pa IN CRex s}
+    /\ isafe s' {pa | MEM pa IN CRex s'}
+    /\ (!r. r IN CR s ==> (Cv s r = Cv s' r))
+        ==>
+    (Icode s <=> Icode s')
+``,
+  REPEAT STRIP_TAC >>
+  ASSUME_TAC Inv_spec >>
+  FULL_SIMP_TAC std_ss [] >>
+  IMP_RES_TAC Icode_CR_po 
+);
+
+val Icode_iCoh_oblg = store_thm("Icode_iCoh_oblg", ``
+!s. Icode s ==> iCoh s.ms {pa | MEM pa IN CRex s}
+``,
+  REPEAT STRIP_TAC >>
+  ASSUME_TAC Inv_spec >>
+  FULL_SIMP_TAC std_ss [] >>
+  IMP_RES_TAC Icode_iCoh_po 
+);
+
+val Icode_isafe_oblg = store_thm("Icode_isafe_oblg", ``
+!s. Icode s ==> isafe s {pa | MEM pa IN CRex s}
+``,
+  REPEAT STRIP_TAC >>
+  ASSUME_TAC Inv_spec >>
+  FULL_SIMP_TAC std_ss [] >>
+  IMP_RES_TAC Icode_isafe_po 
+);
+
 val Icm_oblg = store_thm("Icm_oblg", ``
 !s s'. Inv s /\ drvbl s s' ==> Icm s'
 ``,
@@ -198,9 +276,16 @@ val Icm_oblg = store_thm("Icm_oblg", ``
 ); 
 
 val Inv_oblg = store_thm("Inv_oblg", ``
-!s. Inv s ==> Ifun s /\ Icoh s /\ Icm s
+!s. Inv s <=> Ifun s /\ Icoh s /\ Icode s /\ Icm s
 ``,
   REPEAT STRIP_TAC >>
   ASSUME_TAC Inv_spec >>
   FULL_SIMP_TAC std_ss []
 ); 
+
+
+(*********** finish ************)
+
+val _ = export_theory();
+
+
